move make_path to bfs, ultimately make_solution should depend on it

print_solution.ml
@@ -1,11 +1,17 @@
 open All_positions
 
+let code_to_direction d =
+  let (_, v) = Uint63.to_int2 d in
+  if v = 1 then "up\n" else if v = 2 then "right\n" else
+  if v = 3 then "down\n" else if v = 4 then "left\n" else "";;
+
 let rec print_solution = function
   [] -> print_string ""
 | (d, _) :: tl ->
-  let direction = 
-    let (_, v) = Uint63.to_int2 d in
-    if v = 1 then "up\n" else if v = 2 then "right\n" else
-    if v = 3 then "down\n" else if v = 4 then "left\n" else "" in
-  print_string direction; print_solution tl;;
+  print_string (code_to_direction d); print_solution tl;;
+
+let rec print_solution' = function
+  [] -> print_string ""
+| d :: tl ->
+  print_string (code_to_direction d); print_solution' tl;;
 
