print_solution.mli
@@ -4,3 +4,4 @@ open All_positions
    moves are encoded by integers between 1 and 4, 1 = up, 2 = right, 3 = down
    4 = left *)
 val print_solution : (Uint63.t * Uint63.t) list -> unit
+val print_solution': Uint63.t list -> unit
