stub3.ml
@@ -7,8 +7,8 @@ let cached_solutions = (from_channel (open_in "cube.data") :
 
 let anon_fun s =
   let result =
-      make_solution (Uint63.of_int (int_of_string s)) cached_solutions in
-      print_solution result;;
+      make_solution' (Uint63.of_int (int_of_string s)) cached_solutions in
+      print_solution' result;;
 
 let () = Arg.parse [] anon_fun "sorry, no documentation\n";;
 
